theories/Reductions/FMsetC_to_LPolyNC.v
@@ -18,565 +18,123 @@ Require Import List.
 Import ListNotations.
 
 From Undecidability Require Import Problems.LPolyNC Problems.FMsetC Problems.Reduction.
+From Undecidability Require Import FMset.mset_utils.
+From Undecidability Require FMset.mset_eq_utils.
 
-Section Facts.
-
-  (* induction principle wrt. a decreasing measure f *)
-  (* example: elim /(measure_ind length) : l. *)
-  Lemma measure_ind {X: Type} (f: X -> nat) (P: X -> Prop) : 
-    (forall x, (forall y, f y < f x -> P y) -> P x) -> forall (x : X), P x.
-  Proof.
-    apply: well_founded_ind.
-    apply: Wf_nat.well_founded_lt_compat. move=> *. by eassumption.
-  Qed.
-
-  (* transforms a goal (A -> B) -> C into goals A and B -> C *)
-  Lemma unnest {A B C: Prop} : A -> (B -> C) -> (A -> B) -> C.
-  Proof. auto. Qed.
-
-  Lemma unnest_t (X Y Z: Type): X -> (Y -> Z) -> (X -> Y) -> Z.
-  Proof. by auto. Qed.
-
-  (* duplicates argument *)
-  Lemma copy {A: Prop} : A -> A * A.
-  Proof. done. Qed.
-
-End Facts.
-
-Section NatNat.
-
-(* 0 + 1 + ... + n *)
-Definition big_sum (n : nat) : nat := nat_rec _ 0 (fun i m => m + (S i)) n.
-
-(* bijection from nat * nat to nat *)
-Definition nat2_to_nat '(x, y) : nat := (big_sum (x + y)) + y.
-
-Definition next_nat2 '(x, y) : nat * nat := if x is S x then (x, S y) else (S y, 0).
-
-(* bijection from nat to nat * nat *)
-Definition nat_to_nat2 (n : nat) : nat * nat := Nat.iter n next_nat2 (0, 0).
-
-Lemma nat_nat2_cancel : cancel nat2_to_nat nat_to_nat2.
-Proof.
-  move=> a. move Hn: (nat2_to_nat a) => n.
-  elim: n a Hn.
-    case; case=> [|?]; case=> [|?]=> /=; by [|lia].
-  move=> n IH [x y]. case: y => [|y] /=. case: x => [|x] //=.
-  all: rewrite ? (Nat.add_0_r, Nat.add_succ_r); case.
-    rewrite -/(nat2_to_nat (0, x)). by move /IH ->.
-  rewrite -/(nat2_to_nat (S x, y)). by move /IH ->.
-Qed.
-
-Lemma nat2_nat_cancel : cancel nat_to_nat2 nat2_to_nat.
-Proof.
-  elim=> //=.
-  move=> n. move: (nat_to_nat2 n) => [+ ?].
-  case=> /= => [|?]; rewrite ? (Nat.add_0_r, Nat.add_succ_r) => /=; by lia.
-Qed.
-
-Lemma nat_to_nat2_non_increasing {n} : fst (nat_to_nat2 n) + snd (nat_to_nat2 n) < S n.
-Proof.
-  elim: n=> [|n] //=.
-  move: (nat_to_nat2 n) => [x y].
-  case: y => [|y]; case: x => [|x] /=; by lia.
-Qed.
-
-
-Inductive tree : Set :=
-  | leaf : tree
-  | node : nat -> tree -> tree -> tree.
-
-Fixpoint tree_to_nat (t: tree) : nat :=
-  match t with
-  | leaf => 0
-  | node n t u => S (nat2_to_nat (n, nat2_to_nat ((tree_to_nat t), (tree_to_nat u))))
+Definition encode_msetc (c : msetc) : polyc :=
+  match c with
+  | msetc_zero x => polyc_one x
+  | msetc_sum x y z => polyc_sum x y z
+  | msetc_h x y => polyc_prod x [0; 1] y
   end.
-
-Lemma aux1 {n} : (fst (nat_to_nat2 (snd (nat_to_nat2 n)))) < S n.
-Proof. 
-  have ? := @nat_to_nat2_non_increasing n.
-  have ? := @nat_to_nat2_non_increasing (snd (nat_to_nat2 n)).
-  by lia.
-Qed.
-
-Lemma aux2 {n} : (snd (nat_to_nat2 (snd (nat_to_nat2 n)))) < S n.
-Proof. 
-  have ? := @nat_to_nat2_non_increasing n.
-  have ? := @nat_to_nat2_non_increasing (snd (nat_to_nat2 n)).
-  by lia.
-Qed.
-  
-Definition nat_to_tree : nat -> tree.
-Proof.
-  apply: (Fix lt_wf _). case.
-    exact (fun _ => leaf).
-  move=> n f.
-  pose m := snd (nat_to_nat2 n).
-  refine (node (fst (nat_to_nat2 n)) (f (fst (nat_to_nat2 m)) _) (f (snd (nat_to_nat2 m)) _)).
-    exact aux1.
-  exact aux2.
-Defined.
-
-Lemma nat_to_tree_S_nP {n} : 
-  nat_to_tree (S n) = 
-    node (fst (nat_to_nat2 n)) 
-      (nat_to_tree (fst (nat_to_nat2 (snd (nat_to_nat2 n)))))
-      (nat_to_tree (snd (nat_to_nat2 (snd (nat_to_nat2 n))))).
-Proof.
-  rewrite /nat_to_tree Fix_eq=> //. elim=> // *. by f_equal.
-Qed.
-    
-Lemma nat_tree_cancel {t} : nat_to_tree (tree_to_nat t) = t.
-Proof.
-  elim: t=> // *.
-  rewrite /tree_to_nat nat_to_tree_S_nP nat_nat2_cancel.
-  rewrite -/tree_to_nat /fst /snd -/(fst _) -/(snd _) nat_nat2_cancel. 
-  by f_equal.
-Qed.
-    
-Lemma tree_nat_cancel {n} : tree_to_nat (nat_to_tree n) = n.
-Proof.
-  elim /lt_wf_ind: n. case=> //.
-  move=> n IH. rewrite nat_to_tree_S_nP /tree_to_nat -/tree_to_nat ? IH.
-    1,2: have ? := @nat_to_nat2_non_increasing n.
-    1,2: have ? := @nat_to_nat2_non_increasing (snd (nat_to_nat2 n)).
-    1,2: by lia.
-  rewrite - surjective_pairing nat2_nat_cancel.
-  by rewrite - surjective_pairing nat2_nat_cancel.
-Qed.
-
-End NatNat.
-
-Fixpoint term_to_tree (t: mset_term) : tree :=
-  match t with
-  | mset_term_zero => leaf
-  | mset_term_var x => node 0 (node x leaf leaf) leaf
-  | mset_term_plus t u => node 1 (term_to_tree t) (term_to_tree u)
-  | mset_term_h t => node 2 (term_to_tree t) leaf
-  end.
-
-Fixpoint tree_to_term (t: tree) : mset_term :=
-  match t with
-  | node 0 (node x leaf leaf) leaf => mset_term_var x
-  | node 1 t u => mset_term_plus (tree_to_term t) (tree_to_term u)
-  | node 2 t leaf => mset_term_h (tree_to_term t)
-  | _ => mset_term_zero
-  end.
-
-Definition term_to_nat (t: mset_term) : nat :=
-  tree_to_nat (term_to_tree t).
-
-Definition nat_to_term (n: nat) : mset_term :=
-  tree_to_term (nat_to_tree n).
-
-Lemma nat_term_cancel {t} : nat_to_term (term_to_nat t) = t.
-Proof.
-  rewrite /nat_to_term /term_to_nat nat_tree_cancel. elim: t.
-  - done.
-  - done.
-  - by move=> t + u /= => -> ->.
-  - by move=> t /= => ->.
-Qed. 
-
-(* decompose mset_term into poly constraints *)
-Fixpoint term_to_polycs (t: mset_term) : list polyc :=
-  match t with
-  | mset_term_zero => [polyc_one (term_to_nat t)]
-  | mset_term_var x => []
-  | mset_term_plus u v => 
-      [polyc_sum (term_to_nat t) (term_to_nat u) (term_to_nat v)] ++ 
-      (term_to_polycs u) ++ (term_to_polycs v)
-  | mset_term_h u => 
-      [polyc_prod (term_to_nat t) [0; 1] (term_to_nat u)] ++ (term_to_polycs u)
-  end.
-
-(* count the number of occurrences of each element up to a bound *)
-Definition mset_to_poly (A: list nat) := 
-  map (fun i => count_occ (Nat.eq_dec) A i) (seq 0 (S (fold_right plus 0 A))).
-
 
 (* encode FMsetC_PROBLEM as LPolyNC_PROBLEM *)
 Definition encode_problem (msetcs : FMsetC_PROBLEM) : LPolyNC_PROBLEM :=
-  flat_map (fun '(t, u) => (polyc_prod (term_to_nat t) [1] (term_to_nat u)) :: term_to_polycs t ++ term_to_polycs u) msetcs.
+  map encode_msetc msetcs.
 
-Definition mset_sat (φ : nat -> list nat) (l : FMsetC_PROBLEM) := 
-  Forall (fun '(A, B) => (mset_sem φ A) ≡ (mset_sem φ B)) l.
+(*
+(* count the number of occurrences of each element up to a bound *)
+Definition mset_to_poly (A: list nat) := 
+  map (fun i => count_occ (Nat.eq_dec) A i) (seq 0 (S (fold_right plus 0 A))).
+*)
 
-Lemma mset_satP {φ l} : mset_sat φ l <-> (forall (A B : mset_term), In (A, B) l -> (mset_sem φ A) ≡ (mset_sem φ B)).
+Fixpoint mset_to_poly (A: list nat) := 
+  match A with
+  | [] => []
+  | a :: A => poly_add (repeat 0 a ++ [1]) (mset_to_poly A)
+  end.
+
+Lemma Forall_mapP {X Y : Type} {P : Y -> Prop} {f : X -> Y} {l : list X} : 
+  Forall P (map f l) <-> Forall (fun x => P (f x)) l.
 Proof.
-  rewrite /mset_sat Forall_forall. constructor.
-  - move=> H A B. apply /H.
-  - move=> H [A B]. apply /H.
-Qed.
+Admitted.
 
-Section ForallNorm.
-
-Variable T : Type.
-Variable P : T -> Prop.
-
-Lemma Forall_nilP : Forall P [] <-> True.
-Proof. by constructor. Qed.
-
-Lemma Forall_consP {a A} : Forall P (a :: A) <-> P a /\ Forall P A.
-Proof.
-  constructor. 
-    move=> H. by inversion H.
-  move=> [? ?]. by constructor.
-Qed.
-
-Lemma Forall_singletonP {a} : Forall P [a] <-> P a.
-Proof. rewrite Forall_consP Forall_nilP. by tauto. Qed.
-
-Lemma Forall_appP {A B}: Forall P (A ++ B) <-> Forall P A /\ Forall P B.
-Proof.
-  elim: A.
-    constructor; by [|case].
-  move=> ? ? IH /=. rewrite ? Forall_consP ? IH.
-  by tauto.
-Qed.
-
-(* usage rewrite ? Forall_norm *)
-Definition Forall_norm := (@Forall_appP, @Forall_singletonP, @Forall_consP, @Forall_nilP).
-
-End ForallNorm.
-
-
-Lemma Forall_flat_mapP {X Y: Type} {P: Y -> Prop} {f: X -> list Y} {A: list X}: 
-  Forall P (flat_map f A) <-> Forall (fun a => Forall P (f a)) A.
-Proof.
-  elim: A.
-    move=> /=. by constructor.
-  move=> a A IH. by rewrite /flat_map -/(flat_map _ _) ? Forall_norm IH.
-Qed.
-
-Lemma mset_poly_appP {A B} : mset_to_poly (A ++ B) ≃ poly_add (mset_to_poly A) (mset_to_poly B).
+Lemma mset_to_poly_eqI {A B} : A ≡ B -> mset_to_poly A ≃ mset_to_poly B.
 Proof. Admitted.
 
-Lemma mset_poly_mapP {A} : mset_to_poly (map S A) ≃ poly_mult [0; 1] (mset_to_poly A).
+Lemma mset_to_poly_appP {A B} : mset_to_poly (A ++ B) ≃ poly_add (mset_to_poly A) (mset_to_poly B).
+Proof. Admitted. 
+
+Lemma mset_to_poly_mapP {A} : mset_to_poly (map S A) ≃ 0 :: mset_to_poly A.
 Proof. Admitted.
 
-Lemma mset_poly_eqP {A B} : A ≡ B -> mset_to_poly A ≃ poly_mult [1] (mset_to_poly B).
+Lemma poly_eq_trans {p q r} : p ≃ q -> q ≃ r -> p ≃ r.
+Proof. Admitted.
+
+Lemma map_0P {X: Type} {A: list X} : (map (fun=> 0) A) = repeat 0 (length A).
+Proof. Admitted.
+
+Lemma poly_add_0P {n p} : poly_add (repeat 0 n) p = p.
+Proof. Admitted.
+
+Lemma poly_add_comm {p q} : poly_add p q = poly_add q p.
 Proof. Admitted.
 
 Lemma completeness {l} : FMsetC_SAT l -> LPolyNC_SAT (encode_problem l).
 Proof.
-  move=> [φ]. rewrite -mset_satP => Hφ.
-  pose ψ x := mset_to_poly (mset_sem φ (nat_to_term x)).
-  have Hψ (A) : Forall (polyc_sem ψ) (term_to_polycs A).
-  {
-    elim: A.
-    - by rewrite /term_to_polycs ? Forall_norm /ψ /polyc_sem nat_term_cancel.
-    - by rewrite /term_to_polycs.
-    - move=> A IHA B IHB. 
-      rewrite /term_to_polycs -/term_to_polycs ? Forall_norm.
-      constructor; first last.
-        by constructor.
-      rewrite /ψ /polyc_sem ? nat_term_cancel.
-      rewrite /(mset_sem _ (mset_term_plus _ _)) -/mset_sem - ? /(polyc_sem _).
-      by apply: mset_poly_appP.
-    - move=> A IH. 
-      rewrite /term_to_polycs -/term_to_polycs ? Forall_norm.
-      constructor; last done.
-      rewrite /ψ /polyc_sem ? nat_term_cancel.
-      rewrite /(mset_sem _ (mset_term_h _)) -/mset_sem.
-      by apply: mset_poly_mapP.
-  }
-  exists ψ.
-  rewrite - Forall_forall /encode_problem Forall_flat_mapP.
-  apply: Forall_impl; last eassumption. 
-  move=> [A B]. rewrite ? Forall_norm.
-  move=> HφAB. constructor; first last.
-    by constructor.
-  apply: mset_poly_eqP. by rewrite ? nat_term_cancel.
+  move=> [φ]. rewrite -Forall_forall => Hφ.
+  exists (fun x => mset_to_poly (φ x)). rewrite -Forall_forall.
+  rewrite /encode_problem. rewrite Forall_mapP.
+  apply: Forall_impl; last by eassumption. case.
+  - move=> x /=. by move=> /mset_eq_utils.eq_symm /mset_eq_utils.eq_singletonE ->.
+  - move=> x y z /= /mset_to_poly_eqI. move /poly_eq_trans. apply.
+    by apply mset_to_poly_appP.
+  - move=> x y /= /mset_to_poly_eqI. move /poly_eq_trans. apply.
+    move: (φ y) => A. rewrite map_0P. have -> : [0] = repeat 0 1 by done.
+    rewrite [poly_add _ (repeat _ _)] poly_add_comm. rewrite ? poly_add_0P.
+    have -> := map_ext (fun x => x + 0) id Nat.add_0_r. rewrite map_id. 
+    by apply: mset_to_poly_mapP.
 Qed.
-
-Fixpoint mapi {X Y: Type} (f: nat -> X -> Y) i (A: list X) :=
-  match A with
+    
+Fixpoint poly_to_mset (p: list nat) := 
+  match p with
   | [] => []
-  | a :: A => (f i a) :: (mapi f (S i) A)
+  | a :: p => (repeat 0 a) ++ map S (poly_to_mset p)
   end.
-
-(* count the number of occurrences of each element up to a bound *)
-Definition poly_to_mset (p: list nat) := 
-  concat (mapi (fun i a => repeat i a) 0 p).
-
-Lemma poly_add_zeroE {p q} : p ≃ poly_add q [0] -> p ≃ q.
-Proof. Admitted.
 
 Lemma poly_to_mset_eqI {p q} : p ≃ q -> poly_to_mset p ≡ poly_to_mset q.
 Proof. Admitted.
 
-Lemma poly_eq_symm {p q} : p ≃ q -> q ≃ p.
+Lemma poly_to_mset_addP {p q} : poly_to_mset (poly_add p q) ≡ poly_to_mset p ++ poly_to_mset q.
 Proof. Admitted.
-
-Lemma mset_to_poly_eqE {A B} : mset_to_poly A ≃ mset_to_poly B -> A ≡ B.
-Proof. Admitted.
-
-Lemma poly_to_mset_appP {p q} : poly_to_mset (poly_add p q) ≡ poly_to_mset p ++ poly_to_mset q.
-Proof. Admitted.
-
-From Undecidability Require Reductions.H10UC_to_FMsetC.
 
 Lemma soundness {l} : LPolyNC_SAT (encode_problem l) -> FMsetC_SAT l.
 Proof.
-  move=> [ψ]. rewrite -Forall_forall Forall_flat_mapP => Hψ.
-  pose φ x := poly_to_mset (ψ (term_to_nat (mset_term_var x))).
-  exists φ. rewrite -mset_satP.
-  apply: Forall_impl; last by eassumption.
-  move=> [t u]. rewrite ? Forall_norm => [[+ [+]]].
-  rewrite /polyc_sem -/(polyc_sem _) /poly_mult.
-  under map_ext=> n. have -> : 1 * n = n by lia. over.
-  rewrite map_id. move /poly_add_zeroE.
-  rewrite -/(mset_eq _ _).
-
-  have Hφ (s) : Forall (polyc_sem ψ) (term_to_polycs s) -> mset_sem φ s ≡ poly_to_mset (ψ (term_to_nat s)).
-  {
-    clear. elim: s.
-    - rewrite /term_to_polycs ? Forall_norm /polyc_sem /φ /mset_sem.
-      move=> H. have -> : [0] = poly_to_mset [1] by done.
-      apply: poly_to_mset_eqI. by apply: poly_eq_symm.
-    - move=> x _.
-      by rewrite /term_to_polycs ? Forall_norm /polyc_sem /φ /mset_sem.
-    - move=> t IHt u IHu.
-      rewrite /term_to_polycs -/term_to_polycs ? Forall_norm.
-      move=> [+ [/IHt {}IHt /IHu {}IHu]].
-      rewrite /polyc_sem /φ /mset_sem -/mset_sem -/φ.
-      move=> Hψ.
-      under (H10UC_to_FMsetC.eq_lr _ (H10UC_to_FMsetC.eq_refl) (A' := poly_to_mset (ψ (term_to_nat t)) ++ poly_to_mset (ψ (term_to_nat u)))).
-        by apply: H10UC_to_FMsetC.eq_appI.
-      rewrite -/(mset_eq _ _).
-      apply: mset_to_poly_eqE.
-      over.
-  }
-    admit.
-  move=> Htu /Hφ Ht /Hφ Hu.
-  under H10UC_to_FMsetC.eq_lr; [by eassumption |by eassumption | ].
-  rewrite -/(mset_eq _ _). clear Ht Hu.
-  by apply: poly_to_mset_eqI.
-  
-
-
-
-(*
-(* inject mset_term into poly variables *)
-Fixpoint term_to_nat (t: mset_term) : nat :=
-  match t with
-  | mset_term_zero => nat2_to_nat (0, 0)
-  | mset_term_var x => nat2_to_nat (1, x)
-  | mset_term_plus t u => nat2_to_nat (2, nat2_to_nat ((term_to_nat t), (term_to_nat u)))
-  | mset_term_h t => nat2_to_nat (3, term_to_nat t)
-  end.
-
-Fixpoint nat_to_term
-
-(* decompose mset_term into poly constraints *)
-Fixpoint term_to_polycs (t: mset_term) : list polyc :=
-  match t with
-  | mset_term_zero => [polyc_sum (term_to_nat t) (term_to_nat t) (term_to_nat t)]
-  | mset_term_var x => []
-  | mset_term_plus u v => [polyc_sum (term_to_nat t) (term_to_nat u) (term_to_nat v)]
-  | mset_term_h u => [polyc_prod (term_to_nat t) [0; 1] (term_to_nat u)]
-  end.
-
-Definition mset_eq_to_polycs (t u: mset_term) :=
-  [polyc_sum (term_to_nat t) (term_to_nat mset_term_zero) (term_to_nat u); 
-  (polyc_sum (term_to_nat mset_term_zero) (term_to_nat mset_term_zero) (term_to_nat mset_term_zero))].
-
-(* encode FMsetC_PROBLEM as LPolyNC_PROBLEM *)
-Definition encode_problem (msetcs : FMsetC_PROBLEM) : LPolyNC_PROBLEM :=
-  flat_map (fun '(t, u) => mset_eq_to_polycs t u ++ term_to_polycs t ++ term_to_polycs u) msetcs.
-
-Definition mset_sat (φ : nat -> list nat) (l : FMsetC_PROBLEM) := 
-  Forall (fun '(A, B) => (mset_sem φ A) ≡ (mset_sem φ B)) l.
-
-Lemma mset_satP {φ l} : mset_sat φ l <-> (forall (A B : mset_term), In (A, B) l -> (mset_sem φ A) ≡ (mset_sem φ B)).
-Proof.
-  rewrite /mset_sat Forall_forall. constructor.
-  - move=> H A B. apply /H.
-  - move=> H [A B]. apply /H.
+  move=> [ψ]. rewrite -Forall_forall Forall_mapP => Hψ.
+  exists (fun x => poly_to_mset (ψ x)). rewrite -Forall_forall.
+  apply: Forall_impl; last by eassumption. case.
+  - by move=> x /= /poly_to_mset_eqI.
+  - move=> x y z /= /poly_to_mset_eqI. move /mset_eq_utils.eq_trans. apply.
+    by apply: poly_to_mset_addP.
+  - move=> x y /= /poly_to_mset_eqI. move /mset_eq_utils.eq_trans. apply.
+    move: (ψ y) => p. rewrite map_0P. have -> : [0] = repeat 0 1 by done.
+    rewrite [poly_add _ (repeat _ _)] poly_add_comm. rewrite ? poly_add_0P.
+    under map_ext => ?. rewrite Nat.add_0_r. over.
+    by rewrite -/(mset_eq _ _) map_id.
 Qed.
 
-Lemma completeness {l} : FMsetC_SAT l -> LPolyNC_SAT (encode_problem l).
+From Undecidability Require Reductions.H10UC_to_FMsetC.
+
+(* many-one reduction from FMsetC to LPolyNC *)
+Theorem FMsetC_to_LPolyNC : FMsetC_SAT ⪯ LPolyNC_SAT.
 Proof.
-  move=> [φ]. rewrite -mset_satP.
-  rewrite /FMsetC_SAT.
-*)
-
-
-(* list facts *)
-
-Lemma singleton_length {X : Type} {A : list X} : length A = 1 -> exists a, A = [a].
-Proof.
-  case: A.
-    done.
-  move => a A /=. case. move /length_zero_iff_nil => ->. by eexists.
+  exists encode_problem => l. constructor.
+    exact completeness.
+  exact soundness.
 Qed.
 
-Lemma nil_or_ex_max (A : list nat) : A = [] \/ exists a, In a A /\ Forall (fun b => a >= b) A.
-Proof.
-  elim: A.
-    by left.
-  move=> a A. case.
-    move=> ->. right. exists a. split; by [left | constructor].
-  move=> [b [Hb1 Hb2]]. right.
-  case: (le_lt_dec a b)=> ?.
-  - exists b. split; by [right | constructor].
-  - exists a. split.
-      by left.
-    constructor.
-      done.
-    move: Hb2. apply /Forall_impl => ?. by lia.
-Qed.
-
-(* count_occ facts *)
-Lemma count_occ_app {X : Type} {D : forall x y : X, {x = y} + {x <> y}} {A B c}:
-count_occ D (A ++ B) c = count_occ D A c + count_occ D B c.
-Proof.
-  elim: A B.
-    done.
-  move=> a A IH B /=. rewrite IH. by case: (D a c).
-Qed.
-
-Lemma count_occ_cons {X : Type} {D : forall x y : X, {x = y} + {x <> y}} {A a c}:
-count_occ D (a :: A) c = count_occ D (locked [a]) c + count_occ D A c.
-Proof.
-  rewrite /count_occ /is_left -lock. by case: (D a c).
-Qed.
-
-(* In facts *)
-Lemma in_cons_iff : forall {A : Type} {a b : A} {l : list A}, In b (a :: l) <-> (a = b \/ In b l).
-Proof. by constructor. Qed.
-
-(* Forall facts *)
-Lemma Forall_nil_iff {X: Type} {P: X -> Prop} : Forall P [] <-> True.
-Proof. by constructor. Qed.
-
-Lemma Forall_cons_iff {T: Type} {P: T -> Prop} {a l} :
-  Forall P (a :: l) <-> P a /\ Forall P l.
-Proof.
-  constructor. 
-    move=> H. by inversion H.
-  move=> [? ?]. by constructor.
-Qed.
-
-Lemma Forall_singleton_iff {X: Type} {P: X -> Prop} {x} : Forall P [x] <-> P x.
-Proof.
-  rewrite Forall_cons_iff. by constructor; [case |].
-Qed.
-
-Lemma Forall_app_iff {T: Type} {P: T -> Prop} {A B}: Forall P (A ++ B) <-> Forall P A /\ Forall P B.
-Proof.
-  elim: A.
-    constructor; by [|case].
-  move=> ? ? IH /=. rewrite ? Forall_cons_iff ? IH.
-  by tauto.
-Qed.
-
-(* usage: rewrite ? Forall_norm *)
-Definition Forall_norm := (@Forall_app_iff, @Forall_singleton_iff, @Forall_cons_iff, @Forall_nil_iff).
-
-(* Forall2 facts *)
-Lemma Forall2_nil_rE {X Y: Type} {P: X -> Y -> Prop} {A}: Forall2 P A [] -> A = [].
-Proof. move=> H. by inversion H. Qed.
-
-Lemma Forall2_nil_lE {X Y: Type} {P: X -> Y -> Prop} {A}: Forall2 P [] A -> A = [].
-Proof. move=> H. by inversion H. Qed.
-
-Lemma Forall2_lastP {X Y: Type} {P: X -> Y -> Prop} {A B a b}:
-  Forall2 P (A ++ [a]) (B ++ [b]) <-> Forall2 P A B /\ P a b.
-Proof. 
-  elim: A B => /=.
-    move=> B. constructor.
-      elim: B => /=.
-        move=> H. by inversion H.
-      move=> c B IH H. inversion H. subst.
-      have := Forall2_nil_lE ltac:(eassumption). by move /app_eq_nil => [_].
-    move=> [/Forall2_nil_lE ->] ? /=. by constructor.
-  move=> c A IH. elim=> /=.
-    constructor.
-      move=> H. inversion H. subst.
-      have := Forall2_nil_rE ltac:(eassumption). by move /app_eq_nil => [_].
-    by move=> [/Forall2_nil_rE].
-  move=> d B IH2. constructor.
-    move=> H. inversion H. subst. constructor.
-      constructor.
-        done.
-      have := iffLR (IH B) ltac:(eassumption). by case.
-    have := iffLR (IH B) ltac:(eassumption). by case.
-  move=> [H ?]. inversion H. subst. constructor.
-    done.
-  apply /IH. by constructor.
-Qed.
-
-(* seq facts *)
-Lemma seq_last start length : seq start (S length) = (seq start length) ++ [start + length].
-Proof.
-  have -> : S length = length + 1 by lia.
-  by rewrite seq_app.
-Qed.
-
-(* repeat facts *)
-Lemma repeat_add {X : Type} {x : X} {m n} : repeat x (m + n) = repeat x m ++ repeat x n.
-Proof.
-  elim: m.
-    done.
-  move=> m IH. cbn. by f_equal.
-Qed.
-
-Lemma Forall_repeat {X: Type} {a} {A: list X} : Forall (fun b => a = b) A -> A = repeat a (length A).
-Proof.
-  elim: A.
-    done.
-  move=> b A IH. rewrite Forall_norm => [[? /IH ->]]. subst b.
-  cbn. by rewrite repeat_length.
-Qed.
-
-
-
-(* encode a single H10UC constraint as a list of FMsetC constraints *)
-Definition encode_h10uc '(x, y, z) := encode_constraint x y z.
-
-(* many-one reduction from H10UC to FMsetC *)
-Theorem H10UC_to_FMsetC : H10UC_SAT ⪯ FMsetC_SAT.
-Proof.
-  exists (fun h10ucs => flat_map encode_h10uc h10ucs).
-  move=> h10ucs. constructor.
-  - move=> [φ Hφ]. 
-    exists (construct_valuation φ).
-    elim: h10ucs Hφ.
-      done.
-    move=> [[x y] z] h10cs IH.
-    move /Forall_forall. rewrite Forall_cons_iff. move=> [Hxyz /Forall_forall /IH].
-    move=> {}IH A B.
-    rewrite /flat_map -/(flat_map _) in_app_iff. case; first last.
-      by apply /IH.
-    rewrite /encode_h10uc.
-    have := @encode_constraint_sat φ x y z ltac:(done).
-    rewrite /mset_sat Forall_forall. by apply.
-  - move=> [φ]. rewrite - mset_satP /mset_sat. move=> Hφ.
-    pose ψ := (fun x => length (φ (embed (x, 0, 1)))).
-    exists ψ.
-    rewrite - Forall_forall.
-    elim: h10ucs Hφ.
-      done.
-    move=> [[x y] z] h10ucs IH. rewrite /flat_map -/(flat_map _) Forall_app_iff.
-    rewrite /(encode_h10uc _).
-    move=> [/encode_constraint_spec Hxyz /IH ?].
-    by constructor.
-Qed.
-
-Check H10UC_to_FMsetC.
-(* Print Assumptions H10UC_to_FMsetC. *)
+Check FMsetC_to_LPolyNC.
+Print Assumptions FMsetC_to_LPolyNC.
 
 From Undecidability Require Import Problems.TM.
-From Undecidability Require Import Reductions.H10C_to_H10UC.
+From Undecidability Require Reductions.H10UC_to_FMsetC.
 
-(* undecidability of FMsetC *)
-Theorem FMsetC_undec : Halt ⪯ FMsetC_SAT.
+(* undecidability of LPolyNC *)
+Theorem LPolyNC_undec : Halt ⪯ LPolyNC_SAT.
 Proof.
-  apply (reduces_transitive H10UC_undec).
-  apply H10UC_to_FMsetC.
+  apply (reduces_transitive H10UC_to_FMsetC.FMsetC_undec).
+  apply FMsetC_to_LPolyNC.
 Qed.
 
-Check FMsetC_undec.
-(* Print Assumptions FMsetC_undec. *)
+Check LPolyNC_undec.
+Print Assumptions LPolyNC_undec.
